formal/Mcmc.lean
@@ -47,6 +47,7 @@ import Mcmc.Executable.Finite.Program
 import Mcmc.Executable.Finite.CompilerIR
 import Mcmc.Executable.Finite.CompilerIRInterpreter
 import Mcmc.Executable.IRFormat
+import Mcmc.Executable.ComposableIR
 import Mcmc.Executable.Finite.IRTests
 import Mcmc.Executable.Primitive
 import Mcmc.Executable.IR
